lib/Lib.RandomSequence.fsti
@@ -6,14 +6,16 @@ open Lib.ByteSequence
 
 
 ///
-/// This module uses the OCaml cryptokit package to provide System randomness
+/// This module uses the OCaml cryptokit package to provide Hardware randomness
+/// (Currently only usable from platforms that support RDRAND)
 ///
 
 val entropy: Type0
+val entropy0: entropy
 
 
-val crypto_random: len:size_nat -> Tot (option (lbytes len))
+val crypto_random: entropy -> len:size_nat -> Tot (entropy & lbytes len)
 
-val crypto_random2: entropy -> len:size_nat -> Tot (entropy & lbytes len)
+val unsound_crypto_random1: len:size_nat -> Tot (option (lbytes len))
 
-val crypto_random3: len:size_nat -> Tot (lbytes len)
+val unsound_crypto_random2: len:size_nat -> Tot (lbytes len)
